feat: BSTree spec as Set

lean/TestingAeneas/BSTree.lean
@@ -1,9 +1,12 @@
 import TestingAeneas.Definitions
-
 import Aeneas
+
 open Aeneas.Std
 
-namespace Spec
+attribute [-simp] Bool.exists_bool
+
+namespace TreeImpl/- {{{ -/
+namespace Spec/- {{{ -/
 
 inductive BSTree(α: Type) where
 | Nil : BSTree α
@@ -45,12 +48,11 @@ inductive BSTree.WellFormed[LE α][DecidableLE α][BoundedOrder α]: BSTree α -
     (non_empty: between l r v)
     : (left_wf: left.WellFormed l v) -> (right_wf: right.WellFormed v r) -> (Node v left right).WellFormed l r
 
-end Spec
-
-namespace Lemmas
+end Spec/- }}} -/
+namespace Lemmas/- {{{ -/
 open testing_aeneas
 
-section Translation
+section Translation/- {{{ -/
 
 @[simp]
 def toSpec: BSTree α -> Spec.BSTree α
@@ -73,7 +75,7 @@ theorem toSpec_equiv{tree tree': BSTree α}
         intro; split_conj <;> apply toSpec_equiv.mp <;> simp [*]
       case mpr =>
         intro ⟨h1, h2⟩; subst h1 h2; simp
-end Translation
+end Translation/- }}} -/
 
 instance: BoundedOrder (Scalar ty) where
   top := ⟨Scalar.max ty, by scalar_tac, by scalar_tac⟩
@@ -110,7 +112,6 @@ theorem for_all_iff_contains[BEq α][LawfulBEq α]{tree: Spec.BSTree α}{p: α -
 
 
 
-@[pspec]
 theorem contains_spec(tree: BSTree Isize)(target: Isize)
 : (toSpec tree).WellFormed l r
 -> ∃ b,
@@ -178,8 +179,7 @@ theorem nil_of_wellformed_of_gt[BEq α][LawfulBEq α][LE α][DecidableLE α][IsT
     simp at *; contradiction
     
 
-@[pspec]
-theorem insert_spec[BEq Isize][LawfulBEq Isize](tree: BSTree Isize)(value: Isize)
+theorem insert_spec(tree: BSTree Isize)(value: Isize)
 : (toSpec tree).WellFormed l r 
 -> ∃ tree',
     BSTreeIsize.insert tree value = Result.ok tree' ∧
@@ -188,11 +188,11 @@ theorem insert_spec[BEq Isize][LawfulBEq Isize](tree: BSTree Isize)(value: Isize
 := by
   intro well_formed
   rw [BSTreeIsize.insert]
-  match tree with
-  | .Nil => 
+  cases tree
+  case Nil => 
     simp [toSpec, Spec.BSTree.insert]
     apply Spec.BSTree.WellFormed.isEmpty
-  | .Node curr left right =>
+  case Node curr left right =>
     simp [toSpec, Spec.BSTree.insert]
     simp [toSpec] at well_formed
     obtain _|⟨_, _, _, left_inv, right_inv, nonempty, left_wf, right_wf⟩ := well_formed 
@@ -208,7 +208,6 @@ theorem insert_spec[BEq Isize][LawfulBEq Isize](tree: BSTree Isize)(value: Isize
       have: (value: Int) <= ↑r := by scalar_tac
       simp [maxOfLe, this]
       apply Spec.BSTree.WellFormed.isCompound
-      -- I'm now getting some really slow updates which are a PITA
       case left_inv => 
         apply for_all_iff_contains.mpr
         intro x x_in_left
@@ -254,4 +253,238 @@ theorem insert_spec[BEq Isize][LawfulBEq Isize](tree: BSTree Isize)(value: Isize
       case right_wf => assumption
       case left_wf => assumption
       case non_empty => simp [Spec.between, minOfLe]; scalar_tac
-end Lemmas
+end Lemmas/- }}} -/
+end TreeImpl/- }}} -/
+
+namespace SetImpl/- {{{ -/
+namespace Spec/- {{{ -/
+/-
+In this case, the spec is simply Mathlib's `Set`.
+Then `insert x` is just `∪ {x}` and `contains`
+is the ∈ operator.
+
+EDIT: Actually, I'll just use a list, with a couple
+ of restrictions if needed
+-/
+/- structure Set(α: Type)where -/
+/-   toList: List α -/
+
+/- def Set.all(condition: α -> Bool)(set : Set α): Bool := set.toList.all condition -/
+
+/- def Set.contains[BEq α](set: Set α)(target: α): Bool := set.toList.contains target -/
+/- instance[BEq α]: Membership (α) (Set α) where mem set target := set.contains target = true -/
+/- instance[BEq α](set: Set α): Decidable (x ∈ set) -/
+
+/- def Set.inclusion[BEq α](set set': Set α): Bool := set.all set'.contains -/
+/- instance[BEq α]: HasSubset (Set α) where Subset set set' := set'.inclusion set = true -/
+
+/- def Set.beq[BEq α](set set': Set α): Bool := set.inclusion set' && set'.inclusion set -/
+/- instance[BEq α]: BEq (Set α) where beq := Set.beq -/
+
+/- def Set.insert[BEq α](set: Set α)(target: α) := -/ 
+/-   if set.all (· != target) -/ 
+/-   then {set with toList := target :: set.toList} -/
+/-   else set`Finset` -/
+
+/- theorem all_contains[BEq α](set: Set α)(condition: α -> Bool) -/
+/- : set.all condition ↔ (∀ x, set.contains x -> condition x) -/ 
+/- := sorry -/
+/- 
+EDIT2: I'm going to try with Mathlib's `Set` again
+-/
+
+
+end Spec/- }}} -/
+
+namespace Lemmas/- {{{ -/
+@[simp]
+abbrev between[LE α][DecidableLE α](lo hi value: α) := decide (lo <= value ∧ value <= hi)
+
+open testing_aeneas
+section Translation/- {{{ -/
+
+@[simp] def toSpec: BSTree α -> Set α
+| .Nil => ∅
+| .Node v left right => {v} ∪ (toSpec left) ∪ (toSpec right)
+
+instance: Coe (BSTree α) (Set α) where
+  coe := toSpec
+
+/- theorem toSpec_equiv{tree tree': BSTree α} -/
+/- : (tree : Set α) = tree' ↔ tree = tree' -/
+/- := sorry -/
+-- NOTE: This refinement is not injective!
+end Translation/- }}} -/
+
+def BSTree.for_all(condition: α -> Bool): BSTree α -> Bool
+| .Nil => true
+| .Node curr left right => condition curr && BSTree.for_all condition left && BSTree.for_all condition right
+
+@[simp]
+theorem for_all_spec{tree: BSTree α}{condition: α -> Bool}
+: BSTree.for_all condition tree ↔ (∀ x ∈ (tree: Set α), condition x)
+:= by 
+  cases tree
+  case Nil => simp [BSTree.for_all, toSpec]
+  case Node curr left right =>
+    simp [BSTree.for_all, toSpec]
+    apply Iff.intro
+    case mp =>
+      intro ⟨curr_cond, left_forall, right_forall⟩
+      simp [for_all_spec] at left_forall right_forall
+      intro x cond
+      /- cases cond <;> simp [*] -- Why doesn't this work? -/
+      match cond with
+      | .inl (.inl h) => simp [*]
+      | .inl (.inr h) => simp [*]
+      | .inr h => simp [*]
+    case mpr =>
+      intro hypot
+      split_conjs
+      · apply hypot; simp
+      · apply for_all_spec.mpr; intro x x_in_left; apply hypot; simp [*]
+      · apply for_all_spec.mpr; intro x x_in_left; apply hypot; simp [*]
+
+@[simp] def well_formed[LE α][DecidableLE α](l r: α): BSTree α -> Prop
+| .Nil => True
+| .Node curr left right =>
+  well_formed l curr left ∧ well_formed curr r right ∧ 
+    BSTree.for_all (between l curr) left ∧
+    BSTree.for_all (between curr r) right  ∧
+    between l r curr
+    
+
+@[pspec]
+theorem contains_spec(tree: BSTree Isize)(target: Isize)
+: well_formed l r tree 
+-> ∃ b,
+    BSTreeIsize.contains tree target = Result.ok b ∧
+    (b = true ↔ target ∈ (tree : Set Isize))
+:= by 
+  intro well_formed
+  rw [BSTreeIsize.contains]
+  match tree with
+  | .Nil => simp
+  | .Node curr left right => 
+    simp 
+    simp at well_formed
+    have ⟨left_wf, right_wf, left_inv, right_inv, nonempty⟩ := well_formed
+    split
+    case isTrue curr_eq_target =>
+      simp [curr_eq_target]
+    case isFalse curr_neq_target =>
+      split
+      simp [Scalar.eq_equiv _ _ |>.not.mp curr_neq_target]
+      case isTrue target_lt_curr => 
+        progress as ⟨left_contains_target, left_contains_target_spec⟩
+        simp [left_contains_target_spec]
+        have: target ∉ (toSpec right) := by
+          intro target_in_right
+          have ⟨lb, ub⟩:= right_inv target target_in_right
+          /- scalar_tac -- target_lt_curr & lb should close this, no? -/
+          have := Trans.trans target_lt_curr lb
+          scalar_tac
+        simp [this]
+      case isFalse target_ge_curr =>
+        have target_ge_curr := (le_of_not_gt target_ge_curr)
+        progress as ⟨right_contains_target, right_contains_target_spec⟩
+        simp [right_contains_target_spec, curr_neq_target]
+        have: target ∉ (toSpec left) := by
+          intro target_in_left
+          have ⟨lb, ub⟩:= left_inv target target_in_left
+          have: curr < (target: Int) := by scalar_tac
+          /- scalar_tac -- target_lt_curr & lb should close this, no? -/
+          have := Trans.trans ub this
+          scalar_tac
+        simp [this]
+
+theorem nil_of_wellformed_of_gt[BEq α][LawfulBEq α][LE α][DecidableLE α][IsTrans α (·≤·)][BoundedOrder α](tree: BSTree α)
+: ¬ (l <= r) -> well_formed l r tree -> tree = .Nil
+:= by
+  intro l_gt_r
+  intro tree_wf
+  match tree with
+  | .Nil => rfl
+  | .Node .. =>
+    have ⟨left_inv, right_inv, left_wf, right_wf, non_empty⟩ := tree_wf
+    simp at non_empty
+    have ⟨lb, ub⟩ := non_empty
+    have: l <= r := Trans.trans lb ub
+    simp at *; contradiction
+
+@[pspec]
+theorem insert_spec(tree: BSTree Isize)(value: Isize)
+: well_formed l r tree
+-> ∃ tree',
+    BSTreeIsize.insert tree value = Result.ok tree' ∧
+    insert value (toSpec tree) = ↑tree' ∧
+    well_formed (minOfLe.min l value) (maxOfLe.max r value) tree'
+:= by
+  intro well_formed
+  rw [BSTreeIsize.insert]
+  cases tree
+  case Nil => simp
+  case Node curr left right =>
+    simp
+    have ⟨left_wf, right_wf, left_inv, right_inv, nonempty⟩ := well_formed 
+    simp at nonempty left_inv right_inv
+    split
+    case isTrue value_lt_curr =>
+      progress as ⟨left', left'_spec, left'_wf⟩
+      simp; split_conjs
+      · rw [<-left'_spec]
+        sorry
+      · simp [maxOfLe, le_of_lt value_lt_curr] at left'_wf
+        assumption
+      · have: value < (r : Int) := Trans.trans value_lt_curr nonempty.right
+        simp [minOfLe, le_of_lt this]
+        assumption
+      · rw [<-left'_spec]
+        simp [le_of_lt value_lt_curr]
+        intro x x_in_left
+        have⟨_, _⟩ := left_inv x x_in_left
+        split_conjs 
+        · left; assumption
+        · assumption
+      · intro x x_in_right
+        have⟨_, _⟩ := right_inv x x_in_right
+        split_conjs 
+        · assumption
+        · left; assumption
+      · right; apply le_of_lt; assumption
+      · left; exact nonempty.right
+    case isFalse not_value_lt_curr =>
+      split
+      case isTrue value_gt_curr =>
+        progress as ⟨right', right'_spec, right'_wf⟩
+        simp; split_conjs
+        · rw [<-right'_spec]
+          sorry
+        · have := Trans.trans nonempty.left value_gt_curr
+          simp [minOfLe, le_of_lt this]
+          assumption
+        · simp [maxOfLe, le_of_lt value_gt_curr] at right'_wf
+          assumption
+        · intro x x_in_left
+          have⟨_, _⟩ := left_inv x x_in_left
+          split_conjs 
+          · left; assumption
+          · assumption
+        · rw [<-right'_spec]
+          simp [le_of_lt value_gt_curr]
+          intro x x_in_right
+          have⟨_, _⟩ := right_inv x x_in_right
+          split_conjs 
+          · assumption
+          · left; assumption
+        · left; exact nonempty.left
+        · left; exact nonempty.right
+      case isFalse not_value_gt_curr =>
+        have: curr = value := by scalar_tac
+        subst this
+        simp [maxOfLe, minOfLe, nonempty]
+        split_conjs <;> assumption
+
+
+end Lemmas/- }}} -/
+end SetImpl/- }}} -/
